dimsum_examples/iris/echo.v
@@ -1,0 +1,437 @@
+From iris.bi.lib Require Import fixpoint.
+From iris.proofmode Require Import proofmode.
+
+Section bi_loop.
+  Context {PROP : bi} {A : Type} (body : (A → PROP) → (A → PROP)).
+
+  Definition bi_loop_pre (bi_loop : leibnizO A -d> PROP) :
+    leibnizO A -d> PROP := λ a,
+    (∀ Φ, □ (∀ x, bi_loop x -∗ Φ x) -∗ body Φ a)%I.
+
+  Global Instance bi_loop_pre_ne n:
+    Proper ((dist n ==> dist n) ==> dist n ==> dist n) bi_loop_pre.
+  Proof.
+    move => ?? Hsim ?? ->. rewrite /bi_loop_pre.
+    repeat (f_equiv || eapply Hsim || reflexivity).
+  Qed.
+
+  Lemma bi_loop_pre_mono loop1 loop2:
+    ⊢ □ (∀ a, loop1 a -∗ loop2 a)
+    → ∀ a , bi_loop_pre loop1 a -∗ bi_loop_pre loop2 a.
+  Proof.
+    iIntros "#Hinner" (a) "Hsim". iIntros (?) "#HC".
+    iApply "Hsim". iIntros "!>" (?) "?". iApply "HC". by iApply "Hinner".
+  Qed.
+
+  Local Instance bi_loop_pre_monotone :
+    BiMonoPred bi_loop_pre.
+  Proof.
+    constructor.
+    - iIntros (Π Ψ ??) "#Hinner". iIntros (?) "Hsim" => /=. iApply bi_loop_pre_mono; [|done].
+      iIntros "!>" (?) "HΠ". by iApply ("Hinner" $! _).
+    - move => bi_loop Hsim n a1 a2 /= ?.
+      apply bi_loop_pre_ne; eauto. move => ??? /=. by apply: Hsim.
+  Qed.
+End bi_loop.
+
+Definition bi_loop {PROP : bi} {A} (body : (A → PROP) → (A → PROP)) (a : A) :=
+  bi_greatest_fixpoint (bi_loop_pre body) a.
+
+Section bi_loop.
+  Context {PROP : bi} {A : Type} (body : (A → PROP) → (A → PROP)).
+
+  Local Existing Instance bi_loop_pre_monotone.
+  Lemma bi_loop_eq a:
+    bi_loop body a ⊣⊢ bi_loop_pre body (bi_loop body) a.
+  Proof. rewrite /bi_loop. apply: greatest_fixpoint_unfold. Qed.
+
+  Lemma bi_loop_step a:
+    (∀ Φ, □ (∀ a, bi_loop body a -∗ Φ a) -∗ body Φ a) ⊢ bi_loop body a.
+  Proof. by rewrite bi_loop_eq. Qed.
+
+  Lemma bi_loop_unfold a:
+    bi_loop body a ⊢ body (bi_loop body) a.
+  Proof. rewrite bi_loop_eq. iIntros "Hl". iApply "Hl". iIntros "!>" (?) "$". Qed.
+End bi_loop.
+
+From dimsum.examples.iris Require Import asm rec2.
+Set Default Proof Using "Type".
+
+Local Open Scope Z_scope.
+
+(* TODO: upstream? *)
+Arguments subst_static _ !_ /.
+
+
+Definition echo_rec : fndef := {|
+  fd_args := [];
+  fd_static_vars := [];
+  fd_vars := [];
+  fd_body := LetE "c" (rec.Call (Val (ValFn "getc")) []) $
+             LetE "_" (rec.Call (Val (ValFn "putc")) [Var "c"]) $
+             rec.Call (Val (ValFn "echo")) [];
+  fd_static := I
+|}.
+Definition echo_prog : gmap string fndef :=
+  <["echo" := echo_rec]> $ ∅.
+
+Section echo.
+  Context `{!dimsumGS Σ} `{!recGS Σ}.
+
+  Lemma sim_echo Π :
+    "echo" ↪ Some echo_rec -∗
+    rec_fn_spec_hoare Tgt Π "echo" (λ es POST0, ⌜es = []⌝ ∗
+      bi_loop (λ LOOP _,
+        rec_fn_spec_hoare Tgt Π "getc" (λ es POST,
+          ⌜es = []⌝ ∗
+        POST (λ c,
+        rec_fn_spec_hoare Tgt Π "putc" (λ es POST,
+          ⌜es = [Val c]⌝ ∗
+        POST (λ _,
+          LOOP tt
+        ))))) tt).
+  Proof.
+    iIntros "#?". iApply rec_fn_spec_hoare_ctx. iIntros "#?".
+    set BODY := (X in bi_loop X).
+    iApply ord_loeb; [done|]. iIntros "!> #IH".
+    iIntros (es Φ). iDestruct 1 as (->) "HΦ".
+    iApply sim_tgt_rec_Call_internal. 2: { done. } { done. }
+    iModIntro => /=.
+    iApply sim_tgt_rec_AllocA; [by econs|] => /=. iIntros (?) "?".
+    destruct ls as [|] => //=. iModIntro.
+    iDestruct (bi_loop_unfold with "HΦ") as "HΦ".
+    iApply (sim_gen_expr_bind _ [LetECtx _ _] with "[-]") => /=.
+    iApply "HΦ". iSplit!. iIntros (?) "HΦ".
+    iApply sim_tgt_rec_LetE. iIntros "!>" => /=.
+    iApply (sim_gen_expr_bind _ [LetECtx _ _] with "[-]") => /=.
+    iApply "HΦ". iSplit!. iIntros (?) "HΦ".
+    iApply sim_tgt_rec_LetE. iIntros "!>" => /=.
+    iApply "IH". iSplit!.
+  Qed.
+
+End echo.
+
+(* Call with direct return *)
+Definition TCallRet {S} (f : string) (vs : list val) (h : heap_state) :
+  spec rec_event S (val * heap_state) :=
+  TVis (Outgoing, ERCall f vs h);;
+  e ← TExist _;
+  TVis (Incoming, e);;
+  if e is ERReturn v h' then
+    TRet (v, h')
+  else
+    TUb.
+
+Definition echo_spec_body : spec rec_event unit unit :=
+  h ← TExist _;
+  '(c, h') ← TCallRet "getc" [] h;
+  TAssume (h = h');;
+  h ← TExist _;
+  '(_, h') ← TCallRet "putc" [c] h;
+  TAssume (h = h');;
+  TRet tt.
+
+Definition echo_spec : spec rec_event unit void :=
+  '(f, vs, h) ← TReceive (λ '(f, vs, h), (Incoming, ERCall f vs h));
+  TAssume (f = "echo");;
+  TAssume (vs = []);;
+  Spec.forever echo_spec_body.
+
+Section echo.
+  Context `{!dimsumGS Σ} `{!recGS Σ}.
+
+  Lemma sim_echo_spec Π γσ_s (σ : m_state (spec_trans _ unit)) :
+    "echo" ↪ Some echo_rec -∗
+    "getc" ↪ None -∗
+    "putc" ↪ None -∗
+    γσ_s ⤳ σ -∗
+    ⌜σ.1 ≡ Spec.forever echo_spec_body⌝ -∗
+    □ switch_external Π (λ _ σ POST,
+        ∃ σ_s, γσ_s ⤳ σ_s ∗
+      POST (spec_trans _ unit) σ_s (λ _ Π',
+      switch Π' (λ κ σ_s' POST,
+       ⌜κ = None⌝ ∗
+      POST Tgt _ (λ σ' Π', ⌜σ' = σ⌝ ∗ ⌜Π' = Π⌝ ∗ γσ_s ⤳ σ_s')))) -∗
+    rec_fn_spec_hoare Tgt Π "echo" (λ es _, ⌜es = []⌝).
+  Proof.
+    iIntros "#?#?#? Hγσ_s Hσ_s #Hswitch". iApply rec_fn_spec_hoare_ctx. iIntros "#?".
+    iIntros (es Φ). iDestruct 1 as %->. iApply sim_echo; [done|]. iSplit!.
+    set BODY := (X in bi_loop X).
+    set EXT := (X in switch_external Π X).
+    iRevert (σ) "Hγσ_s Hσ_s". iApply ord_loeb; [done|]. iIntros "!> #IH".
+    iIntros (σ) "Hγσ_s %". iApply bi_loop_step. iIntros (?) "#HLOOP".
+    iIntros (es ?). iDestruct 1 as (->) "HΦ".
+
+    iApply (fupd_sim_gen_expr with "[-]").
+    iMod (mstate_var_alloc unit) as (γ) "?".
+    iMod (mstate_var_split γ σ.2 with "[$]") as "[Hγ ?]".
+    iModIntro.
+    pose (Hspec := SpecGS γ).
+
+    iApply (sim_tgt_rec_Call_external); [done|].
+    iIntros (???) "Hfns' Hh Ha !>". iIntros (??) "[-> [-> Hσ]]".
+    iApply "Hswitch". iFrame. iSplit!.
+    iIntros (??). iDestruct 1 as (->) "Hs".
+    iApply (sim_gen_expr_intro _ tt with "[Hγ] [-]"); simpl; [done..|].
+    rewrite ->unfold_forever. rewrite {2}/echo_spec_body.
+    rewrite bind_bind. iApply (sim_src_TExist with "[-]").
+    rewrite bind_bind.
+    (* TODO: don't unfold TCallRet *)
+    rewrite /TCallRet bind_bind.
+    iApply sim_gen_TVis. iIntros ([]) "Hγ". iIntros (??) "[-> [-> _]]".
+    iApply "Hs". iSplit!. iIntros (??) "[-> Hs]".
+    iApply (sim_gen_stop with "[-]"). iApply "Hs". iSplit!.
+    iIntros (??) "[-> [-> ?]]".
+    iApply (sim_tgt_rec_Waiting_raw with "[-]"). iSplit.
+    { iIntros. iModIntro. iApply "Hswitch". iFrame. iSplit!.
+      iIntros (??) "[-> Hs]".
+      iApply (sim_gen_expr_intro _ tt with "[Hγ] [-]"); simpl; [done..|].
+      rewrite bind_bind. iApply (sim_src_TExist with "[-]").
+      rewrite bind_bind. iApply sim_gen_TVis.
+      iIntros ([]) "Hγ". iIntros (??) "[-> [-> _]]".
+      iApply "Hs". iSplit!. iIntros (??) "[-> _]".
+      iApply (sim_gen_expr_intro _ tt with "[Hγ] [-]"); simpl; [done..|].
+      iApply sim_src_TUb. }
+    iIntros. iModIntro. iApply "Hswitch". iFrame. iSplit!.
+    iIntros (??) "[-> Hs]".
+    iApply (sim_gen_expr_intro _ tt with "[Hγ] [-]"); simpl; [done..|].
+    rewrite bind_bind. iApply (sim_src_TExist with "[-]").
+    rewrite bind_bind. iApply sim_gen_TVis.
+    iIntros ([]) "Hγ". iIntros (??) "[-> [-> _]]".
+    iApply "Hs". iSplit!. iIntros (??) "[-> Hs]".
+    iApply (sim_gen_expr_intro _ tt with "[Hγ] [-]"); simpl; [done..|].
+    rewrite bind_ret_l bind_bind. iApply (sim_src_TAssume with "[-]").
+    iIntros (<-). iApply sim_gen_expr_None => /=.
+    iIntros (? [] ?) "Hγ". iIntros (??) "[-> [-> _]]".
+    iApply "Hs". iSplit!. iIntros (??) "[-> [-> ?]]".
+    iApply "Hσ". iSplit!. iFrame. iApply "HΦ".
+
+    iIntros (es ?). iDestruct 1 as (->) "HΦ".
+    iApply (sim_tgt_rec_Call_external); [done|].
+    iIntros (???) "Hfns'' Hh Ha !>". iIntros (??) "[-> [-> Hσ]]".
+    iApply "Hswitch". iFrame. iSplit!.
+    iIntros (??). iDestruct 1 as (->) "Hs".
+    iApply (sim_gen_expr_intro _ tt with "[Hγ] [-]"); simpl; [done..|].
+    rewrite bind_bind. iApply (sim_src_TExist with "[-]").
+    rewrite bind_bind.
+    (* TODO: don't unfold TCallRet *)
+    setoid_rewrite bind_bind.
+    iApply sim_gen_TVis. iIntros ([]) "Hγ". iIntros (??) "[-> [-> _]]".
+    iApply "Hs". iSplit!. iIntros (??) "[-> Hs]".
+    iApply (sim_gen_stop with "[-]"). iApply "Hs". iSplit!.
+    iIntros (??) "[-> [-> ?]]".
+    iApply (sim_tgt_rec_Waiting_raw with "[-]"). iSplit.
+    { iIntros. iModIntro. iApply "Hswitch". iFrame. iSplit!.
+      iIntros (??) "[-> Hs]".
+      iApply (sim_gen_expr_intro _ tt with "[Hγ] [-]"); simpl; [done..|].
+      setoid_rewrite bind_bind. iApply (sim_src_TExist with "[-]").
+      setoid_rewrite bind_bind. iApply sim_gen_TVis.
+      iIntros ([]) "Hγ". iIntros (??) "[-> [-> _]]".
+      iApply "Hs". iSplit!. iIntros (??) "[-> _]".
+      iApply (sim_gen_expr_intro _ tt with "[Hγ] [-]"); simpl; [done..|].
+      iApply sim_src_TUb. }
+    iIntros. iModIntro. iApply "Hswitch". iFrame. iSplit!.
+    iIntros (??) "[-> Hs]".
+    iApply (sim_gen_expr_intro _ tt with "[Hγ] [-]"); simpl; [done..|].
+    setoid_rewrite bind_bind. iApply (sim_src_TExist with "[-]").
+    setoid_rewrite bind_bind. iApply sim_gen_TVis.
+    iIntros ([]) "Hγ". iIntros (??) "[-> [-> _]]".
+    iApply "Hs". iSplit!. iIntros (??) "[-> Hs]".
+    iApply (sim_gen_expr_intro _ tt with "[Hγ] [-]"); simpl; [done..|].
+    rewrite bind_ret_l bind_bind. iApply (sim_src_TAssume with "[-]").
+    iIntros (<-). rewrite bind_ret_l. iApply sim_gen_expr_None => /=.
+    iIntros (? [] ?) "Hγ". iIntros (??) "[-> [-> _]]".
+    iApply "Hs". iSplit!. iIntros (??) "[-> [-> ?]]".
+    iApply "Hσ". iSplit!. iFrame. iApply "HΦ". iApply "HLOOP".
+    iApply ("IH" with "[$] [//]").
+  Qed.
+
+  Lemma echo_spec_sim :
+    rec_state_interp (rec_init echo_prog) None -∗
+    (rec_init echo_prog) ⪯{rec_trans, spec_trans rec_event ()} (echo_spec, ()).
+  Proof.
+    iIntros "[#Hfns [Hh Ha]] /=".
+    iApply (fupd_sim with "[-]").
+    iMod (mstate_var_alloc (m_state (spec_trans rec_event ()))) as (γσ_s) "Hγσ_s".
+    iMod (mstate_var_alloc (m_state rec_trans)) as (γσ_t) "Hγσ_t".
+    iMod (mstate_var_alloc (option rec_event)) as (γκ) "Hγκ".
+
+    iMod (mstate_var_alloc unit) as (γs) "?".
+    iMod (mstate_var_split γs tt with "[$]") as "[Hγs ?]".
+    iModIntro.
+    pose (Hspec := SpecGS γs).
+
+    iApply (sim_tgt_constP_intro γσ_t γσ_s γκ with "Hγσ_t Hγσ_s Hγκ [-]"). iIntros "Hγσ_s".
+
+    iApply (sim_tgt_rec_Waiting_raw _ []).
+    iSplit; [|by iIntros].
+    iIntros (f fn vs h ?) "!>".
+    iApply (sim_tgt_constP_elim γσ_t γσ_s γκ with "[Hγσ_s] [-]"); [done..|].
+    iIntros "Hγσ_s Hγσ_t Hγκ".
+
+    iApply (sim_gen_expr_intro _ tt with "[Hγs] [-]"); [simpl; done..|].
+    unfold echo_spec, TReceive.
+    rewrite bind_bind. iApply (sim_src_TExist (_, _, _)).
+    rewrite bind_bind.
+    iApply sim_gen_TVis. iIntros ([]) "Hγs". iIntros (??) "[-> [-> _]]".
+    iApply (sim_src_constP_next with "[Hγσ_t] [Hγκ] [Hγσ_s] [%] [-]"); [done..|].
+    iIntros "Hγσ_s". iApply sim_gen_stop.
+    iApply (sim_tgt_constP_elim γσ_t γσ_s γκ with "[Hγσ_s] [-]"); [done..|].
+    iIntros "Hγσ_s Hγσ_t Hγκ".
+    iApply (sim_gen_expr_intro _ tt with "[Hγs] [-]"); [simpl; done..|].
+    rewrite bind_ret_l.
+    iApply sim_src_TAssume. iIntros (?).
+    iApply sim_src_TAssume. iIntros (?). simplify_eq.
+    iApply sim_gen_expr_None => /=. iIntros (? [] ?) "Hγs".
+    iIntros (??) "[-> [-> _]]".
+
+    iApply (sim_src_constP_next with "[Hγσ_t] [Hγκ] [Hγσ_s] [%] [-]"); [done..|].
+    iIntros "Hγσ_s".
+
+    iApply fupd_sim_gen.
+    iMod (rec_mapsto_alloc_big (h_heap h) with "Hh") as "[Hh _]". { apply map_disjoint_empty_r. }
+    iModIntro.
+
+    iApply (sim_gen_expr_intro _ [] with "[Hh Ha]"). { done. }
+    { rewrite /= /rec_state_interp dom_empty_L right_id_L /=. iFrame "#∗". by iApply rec_alloc_fake. }
+    iApply (sim_gen_expr_bind _ [ReturnExtCtx _] with "[-]") => /=.
+    iApply (sim_echo_spec with "[] [] [] Hγσ_s [//]").
+    1-3: by iApply (rec_fn_intro with "[$]").
+    - iIntros "!>" (??). iDestruct 1 as (?) "[Hγσ_s HC]" => /=.
+      iApply (sim_tgt_constP_elim γσ_t γσ_s γκ with "[Hγσ_s] [-]"); [done..|].
+      iIntros "Hγσ_s Hγσ_t Hγκ".
+      iApply "HC". iSplit!. iIntros (??). iDestruct 1 as (->) "HC".
+      iApply (sim_src_constP_next with "[Hγσ_t] [Hγκ] [Hγσ_s] [%] [-]"); [done..|].
+      iIntros "Hγσ_s".
+      iApply sim_gen_stop.
+      iApply (sim_tgt_constP_elim γσ_t γσ_s γκ with "[Hγσ_s] [-]"); [done..|].
+      iIntros "Hγσ_s Hγσ_t Hγκ".
+      iApply "HC". iSplit!. iIntros (??) "[-> HC]".
+      iApply (sim_src_constP_next with "[Hγσ_t] [Hγκ] [Hγσ_s] [%] [-]"); [done..|].
+      iIntros "Hγσ_s".
+      iApply "HC". iSplit!.
+    - done.
+  Qed.
+
+End echo.
+
+Lemma echo_refines_echo_spec :
+  trefines (rec_mod echo_prog) (spec_mod echo_spec tt).
+Proof.
+  eapply (sim_adequacy #[dimsumΣ; recΣ]); [eapply _..|].
+  iIntros (??) "!>". simpl.
+  iApply (fupd_sim with "[-]").
+  iMod recgs_alloc as (?) "[?[??]]". iModIntro.
+  iApply echo_spec_sim. iFrame.
+Qed.
+
+(*
+  [echo]_rec <= [echo_spec]_spec
+
+  [echo]_rec + [getc]_rec <= ...
+
+getc() = local l [1]; read(l, 1); return l[0]
+
+  [echo]_rec + [putc]_spec <= ...
+
+putc(c) = buffer += [c]; if * then write(buffer, len(buffer)); buffer = []
+
+  ⌜[echo]_rec⌝_r<->a + [getc, putc]_asm <= ...
+
+sales pitch:
+  binary separation logic for multi-language
+  interesting: reuse one spec for many different linking scenarios
+  usuallu in separation logic you are proud that everything is modular,
+   but then there is the assumption that it is implemented in the same language
+   here you can actually swap out the specification for other programs
+  higher-order encoding often uses explicitly that the code is in the same language e.g. with ∀ f, {P} f {Q}
+
+switching:
+  - no obvious that one can do at all
+  - write some notes outside of Coq to explain what it means
+    - with more intuition and less detail
+  -
+ *)
+
+
+
+Definition getc_rec : fndef := {|
+  fd_args := [];
+  fd_static_vars := [];
+  fd_vars := [("l", 1)];
+  fd_body := LetE "c" (rec.Call (Val (ValFn "read")) [Var "l"; Val 1]) $
+             Load (Var "l");
+  fd_static := I
+|}.
+Definition getc_prog : gmap string fndef :=
+  <["getc" := getc_rec]> $ ∅.
+
+Section getc.
+  Context `{!dimsumGS Σ} `{!recGS Σ}.
+
+  Lemma sim_getc Π :
+    "getc" ↪ Some getc_rec -∗
+    rec_fn_spec_hoare Tgt Π "getc" (λ es POST0, ⌜es = []⌝ ∗
+      rec_fn_spec_hoare Tgt Π "read" (λ es POST,
+        ∃ l v, ⌜es = [Val $ ValLoc l; Val $ 1]⌝ ∗ l ↦ v ∗
+      POST (λ _,
+        ∃ c, l ↦ (ValNum c) ∗ POST0 (λ vr, ⌜vr = ValNum c⌝)))).
+  Proof.
+    iIntros "#?".
+    iIntros (es Φ). iDestruct 1 as (->) "HΦ".
+    iApply sim_tgt_rec_Call_internal. 2: { done. } { done. }
+    iModIntro => /=.
+    iApply sim_tgt_rec_AllocA; [by econs|] => /=. iIntros (?) "Hl".
+    destruct ls as [|? []] => //=. 2: iDestruct!. iModIntro.
+    rewrite offset_loc_0. iDestruct "Hl" as "[[Hl _] _]".
+    iApply (sim_gen_expr_bind _ [LetECtx _ _] with "[-]") => /=.
+    iApply "HΦ". iSplit!. iFrame. iIntros (?) "[% [Hl HΦ]]".
+    iApply sim_tgt_rec_LetE. iIntros "!>" => /=.
+    iApply (sim_tgt_rec_Load with "Hl"). iIntros "Hl !>" => /=. iSplit!.
+    iFrame. by iApply "HΦ".
+  Qed.
+
+End getc.
+
+Definition __NR_READ : Z := 0.
+Definition read_addr : Z := 500.
+Definition read_asm : gmap Z asm_instr :=
+  deep_to_asm_instrs read_addr [
+      Amov "R8" __NR_READ;
+      Asyscall;
+      Aret
+    ].
+
+Section read.
+  Context `{!dimsumGS Σ} `{!asmGS Σ}.
+
+  Lemma sim_read Π :
+    ↪ₐ∗ read_asm -∗
+    asm_spec Tgt Π (λ POST0,
+      ∃ ret r8, "PC" ↦ᵣ read_addr ∗ "R30" ↦ᵣ ret ∗ "R8" ↦ᵣ r8 ∗
+    switch Π (λ κ σ POST,
+    POST Tgt asm_trans (λ _ _,
+    POST0 (∃ r8', "PC" ↦ᵣ ret ∗ "R30" ↦ᵣ ret ∗ "R8" ↦ᵣ r8')))).
+  Proof.
+    iIntros "#Hins" (?). iDestruct 1 as (??) "(HPC&HR30&HR8&Hret)".
+    iApply (sim_Jump_internal with "HPC").
+    { iApply (asm_instrs_big_lookup_deep 0 with "[$]"); [lia|simpl; done]. }
+    iIntros "!> HPC" => /=.
+    iApply sim_WriteReg. iSplit.
+    { by iApply learn_regs_done. }
+    iFrame. iIntros "!>" (_ _) "HR8".
+    iApply sim_WriteReg. iSplit.
+    { iApply (learn_regs_reg with "HPC").
+      iApply learn_regs_done. }
+    iFrame. iIntros "!>" (? [-> _]) "HPC".
+
+    iApply (sim_Jump_internal with "HPC").
+    { iApply (asm_instrs_big_lookup_deep 1 with "[$]"); [lia|simpl; done]. }
+    iIntros "!> HPC" => /=.
+    iApply sim_Syscall. iModIntro.
+    iIntros (??). iDestruct 1 as (?? ->) "[? HC]". iApply "HC". iExists _. iSplit.
+    { iApply (learn_regs_reg with "HR8").
+      iApply learn_regs_done. }
+    iIntros ([? _]) "?".
+  Abort.
+End read.
